newLibrary/countMin.dfy
@@ -1,0 +1,124 @@
+// A simple count min library. 
+// methods: 
+// count(key) -- count the key, return updated result
+// events / handlers:
+// query(key) -- query value of key
+// clear(min, max) -- clear indices from min to max
+
+
+include "verifiableLucid.dfy"
+
+
+module CountQuery refines VerifiableLucid {
+
+    datatype Event = 
+        | query(sport : uint8, key : uint32)
+        | response(key : uint32, count : uint32)
+        | clear(i : uint32, j : uint32)
+    
+    // memops
+    function incr (oldVal: uint32, incrBy: uint32) : uint32 { 
+        to_uint32(oldVal + incrBy) 
+    }
+    function memval (oldVal: uint32, unused: uint32) : uint32 { oldVal }
+    function newval (oldVal: uint32, newVal: uint32) : uint32 { newVal }
+
+    class Program ...{
+
+        const nRows : uint32 := 32
+        const seed0 : uint32 := 7
+        const seed1 : uint32 := 13
+
+        var col0 : LArray<uint32>
+        var col1 : LArray<uint32>
+        constructor ()
+            ensures fresh(col0)
+            ensures fresh(col1)
+            ensures col0.cells == zeros(nRows) && col1.cells == zeros(nRows)
+            ensures fresh(this)
+        {
+            col0 := new LArray<uint32>.Create(nRows, 0);
+            col1 := new LArray<uint32>.Create(nRows, 0);
+        }
+
+        function hash(seed : uint32, key : uint32) : uint32
+            ensures 0 <= hash(seed, key) < nRows
+        {
+            to_uint32((seed + key) % nRows)
+        }
+
+        // Increment a key and return current min count
+        method count(key : uint32) returns (result : uint32)          
+            modifies col0`cells, col1`cells
+            requires |col0.cells| == nRows && |col1.cells| == nRows
+            requires col0 != col1
+            // the result is the minimum of the two counts
+            ensures result == 
+                var h0 := hash(seed0, key);
+                var h1 := hash(seed1, key);
+                var count0 := ((  (old(col0.cells)[h0] + 1) % max32));
+                var count1 := ((  (old(col1.cells)[h1] + 1) % max32));
+                if count0 <= count1 then count0 else count1
+            // the arrays are updated correctly
+            ensures             
+                var h0 := hash(seed0, key);
+                var h1 := hash(seed1, key);
+                var count0 := to_uint32(old(col0.cells)[h0] + 1 as uint32);
+                var count1 := to_uint32(old(col1.cells)[h1] + 1 as uint32);
+                LArray.updated_cell(col0, h0, count0)
+                && LArray.updated_cell(col1, h1, count1)
+        {
+            var h0 := hash(seed0, key);
+            var h1 := hash(seed1, key);
+            var count1 := LArray<uint32>.Update(col0, h0, incr, 1, incr, 1);
+            var count2 := LArray<uint32>.Update(col1, h1, incr, 1, incr, 1);
+            if (count1 <= count2) {
+                result := count1;
+            } else {
+                result := count2;
+            }
+        }
+
+        // Query event handler. Generates a response event with the minimum count of the two arrays.
+        method Query(sport : uint8, key : uint32)
+            modifies this`emittedEvents
+            requires readyToHandle(query(sport, key))
+            requires |col0.cells| == nRows && |col1.cells| == nRows
+            requires col0 != col1
+            ensures 
+                var h0 := hash(seed0, key);
+                var h1 := hash(seed1, key);
+                var count0 := old(col0.cells)[h0];
+                var count1 := old(col1.cells)[h1];
+                var count := if count0 <= count1 then count0 else count1;
+                emits(sport, response(key, count))
+        {
+            var h0 := hash(seed0, key);
+            var h1 := hash(seed1, key);
+            var count0 := LArray<uint32>.Get(col0, h0, memval, 0);
+            var count1 := LArray<uint32>.Get(col1, h1, memval, 0);
+            var count := if count0 <= count1 then count0 else count1;
+            generate_port(sport, response(key, count));
+        }
+
+        // Clear event handler. Clears i, then as long as i < j, clears i+1 by generating a recursive event.
+        method Clear(i : uint32, j : uint32)
+            modifies col0`cells, col1`cells
+            modifies this`generatedEvent
+            requires readyToHandle(clear(i, j))
+            requires |col0.cells| == nRows && |col1.cells| == nRows
+            requires col0 != col1
+            requires i < nRows && j < nRows
+            ensures 
+                LArray.updated_cell(col0, i, 0)
+                && LArray.updated_cell(col1, i, 0)
+            ensures i < j ==> generates(clear(i + 1, j))
+        {
+            LArray<uint32>.Set(col0, i, newval, 0);
+            LArray<uint32>.Set(col1, i, newval, 0);
+            if i < j {
+                generate(clear(i + 1, j));
+            }
+        }            
+    }
+}
